Equiv.lean
@@ -27,3 +27,4 @@ import Equiv.Diagonal
 import Equiv.BadRoot
 import Equiv.Recon
 import Equiv.Fuji
+import Equiv.Fill
